\documentclass[fleqn, a4paper, 12pt]{article}
\usepackage{amsmath, amssymb, commath, amsthm}
\usepackage{gensymb}
\usepackage{datetime}
\usepackage{ulem}
\usepackage{enumerate}
\setcounter{secnumdepth}{4}

\newcommand\numberthis{\addtocounter{equation}{1}\tag{\theequation}}

\theoremstyle{definition}
\newtheorem{example}{Example}
\newtheorem{definition}{Definition}

\theoremstyle{theorem}
\newtheorem{theorem}{Theorem}

\newenvironment{solution}
{\begin{proof}[Solution]\let\qed\relax}
	{\end{proof}}
	
%opening
\title{Recitation 7}
\author{}
\date{\formatdate{10}{12}{2014}}

\begin{document}

\maketitle
%\setlength{\mathindent}{0pt}

\tableofcontents

\newpage
\section{}

\begin{example}
	On one side of a boat of mass $M$, a box of mass $m$ is placed and the boat's engine is pulling the box via a massless rope. At $t = 0$ the entire system is at rest. Then the engine is turned on and it starts pulling the box with force $\overrightarrow{F}(t) = \alpha t$ where $\alpha$ is a positive constant. The friction coefficients between the box and the boat are $\mu_s$ and $\mu_k$. The engine is working for time $\tau = \dfrac{mg}{\alpha}$ and then stops. Assuming that the box does not reach the end of the boat nor collide with any other object, what will be the boat's velocity after a very long time $t >> \tau$? Find the box's velocity w.r.t. the boar from the moment the engine is turned on.
\end{example}

\begin{solution}
	\begin{align*}
		F &= \alpha t &;\quad 0 \leq t \leq \tau = \dfrac{mg}{\alpha}\\
		N_s &= \mu_s m g\\
		N_k &= \mu_k m g
	\end{align*}
	Let $t_0$ be the time when the box starts moving.
	\begin{align*}
		F(t) &= \mu_s m g\\
		&= \alpha t\\
		\therefore t_0 &= \dfrac{\mu_s m g}{\alpha}
	\end{align*}
	For $t_0 < t < \tau$,
	\begin{align*}
		\alpha t - \mu_k m g &= m a\\
		\therefore a &= \dfrac{\alpha t}{m} - \mu_k g\\
		\therefore v &= \int\limits_{t_0}^{\tau} a(t) \dif t\\
		&= \dfrac{\alpha}{2m} (\tau^2 - t_0^2) - \mu_k g (\tau - t_0)
	\end{align*}
	For $t > \tau$,
	\begin{align*}
		a &= \mu_k g\\
		\therefore v &= v_{\tau} + \int\limits_{\tau}^{t} g \dif t\\
		&= v_{\tau} - \mu_k g (t - \tau)
	\end{align*}
	
\end{solution}

\end{document}
